theories/Events/State.v
@@ -61,8 +61,12 @@ Section State.
     : itree (stateE +' E) ~> stateT S (itree E)
     := interp_state (case_ h_state pure_state).
 
-  Definition partial_run_state {E F} (h : E +' F ~> stateT S (itree F))
+  Definition later_run_state {E F} (h : E +' F ~> stateT S (itree F))
     : itree (stateE +' E +' F) ~> stateT S (itree F)
+    := interp_state (case_ h_state h).
+
+  Definition partial_run_state {E} (h : E ~> stateT S (itree E))
+    : itree (stateE +' E) ~> stateT S (itree E)
     := interp_state (case_ h_state h).
 
 End State.
